stdlib/closures/theories/closures.v
@@ -1,0 +1,46 @@
+From refinedrust Require Import typing.
+
+
+Definition FnOnce_Params_sig `{RRGS : !(refinedrustGS Σ)} (Self_rt: RT) (Args_rt: RT) (Output_rt: RT) :=
+  (Type).
+Definition FnOnce_Pre_sig `{RRGS : !(refinedrustGS Σ)} (Self_rt: RT) (Args_rt: RT) (Output_rt: RT) (FnOnce_Params: (FnOnce_Params_sig (Self_rt) (Args_rt) (Output_rt))) :=
+  (thread_id → FnOnce_Params → (RT_xt (Self_rt)) → (RT_xt (Args_rt)) → iProp Σ).
+Definition FnOnce_Post_sig `{RRGS : !(refinedrustGS Σ)} (Self_rt: RT) (Args_rt: RT) (Output_rt: RT) (FnOnce_Params: (FnOnce_Params_sig (Self_rt) (Args_rt) (Output_rt))) (FnOnce_Pre: (FnOnce_Pre_sig (Self_rt) (Args_rt) (Output_rt) (FnOnce_Params))) :=
+  (thread_id → FnOnce_Params → (RT_xt (Self_rt)) → (RT_xt (Args_rt)) → (RT_xt (Output_rt)) → iProp Σ).
+Definition FnOnce_PostMut_sig `{RRGS : !(refinedrustGS Σ)} (Self_rt: RT) (Args_rt: RT) (Output_rt: RT) (FnOnce_Params: (FnOnce_Params_sig (Self_rt) (Args_rt) (Output_rt))) (FnOnce_Pre: (FnOnce_Pre_sig (Self_rt) (Args_rt) (Output_rt) (FnOnce_Params))) (FnOnce_Post: (FnOnce_Post_sig (Self_rt) (Args_rt) (Output_rt) (FnOnce_Params) (FnOnce_Pre))) :=
+  (thread_id → FnOnce_Params → (RT_xt (Self_rt)) → (RT_xt (Args_rt)) → (RT_xt (Self_rt)) → (RT_xt (Output_rt)) → iProp Σ).
+Record FnOnce_spec_attrs `{RRGS : !(refinedrustGS Σ)} `{Self_rt : !RT} `{Args_rt : !RT} `{Output_rt : !RT} : Type := mk_FnOnce_spec_attrs {
+  FnOnce_Params  : (FnOnce_Params_sig (Self_rt) (Args_rt) (Output_rt));
+  FnOnce_Pre  : (FnOnce_Pre_sig (Self_rt) (Args_rt) (Output_rt) (FnOnce_Params));
+  FnOnce_Post  : (FnOnce_Post_sig (Self_rt) (Args_rt) (Output_rt) (FnOnce_Params) (FnOnce_Pre));
+  FnOnce_PostMut  : (FnOnce_PostMut_sig (Self_rt) (Args_rt) (Output_rt) (FnOnce_Params) (FnOnce_Pre) (FnOnce_Post));
+}.
+
+#[global] Arguments FnOnce_spec_attrs : clear implicits.
+#[global] Arguments FnOnce_spec_attrs {_ _}.
+#[global] Arguments mk_FnOnce_spec_attrs  {_} {_} {_} {_} {_}.
+
+Section closure_props.
+  Context `{!refinedrustGS Σ}.
+  Context (Clos_rt Args_rt Clos_out_rt : RT).
+
+  Class ClosureHasTrivialPre (fnonce_attrs : FnOnce_spec_attrs Clos_rt Args_rt Clos_out_rt) := closure_has_trivial_pre_proof :
+    ∀ π self args, ⊢ ∃ p, FnOnce_Pre fnonce_attrs π p self args.
+
+End closure_props.
+
+Ltac solve_closure_has_trivial_pre :=
+  match goal with
+  | |- ClosureHasTrivialPre _ _ _ _ =>
+    unfold ClosureHasTrivialPre;
+    intros ???; prepare_initial_coq_context;
+    iStartProof;
+    unshelve (repeat liRStep; solve[fail]);
+    unshelve (sidecond_solver);
+    sidecond_hammer;
+    apply inhabitant
+  end.
+
+(* TODO: don't have this as hint, but generate instances in the frontend *)
+Global Hint Extern 100 (ClosureHasTrivialPre _ _ _ _) =>
+  solve_closure_has_trivial_pre : typeclass_instances.
